lib/coq/Sail_operators_mwords.v
@@ -1,5 +1,7 @@
 Require Import Sail_values.
 Require Import Sail_operators.
+Require Import Prompt_monad.
+Require Import Prompt.
 Require bbv.Word.
 Require Import Arith.
 Require Import Omega.
@@ -37,22 +39,32 @@ Definition access_vec_inc {a} : mword a -> Z -> bitU := access_mword_inc.
 Definition access_vec_dec {a} : mword a -> Z -> bitU := access_mword_dec.
 
 (*val update_vec_inc : forall 'a. Size 'a => mword 'a -> integer -> bitU -> mword 'a*)
-Definition update_vec_inc {a} : mword a -> Z -> bitU -> mword a := update_mword_inc.
+(* TODO: probably ought to use a monadic version instead, but using bad default for
+   type compatibility just now *)
+Definition update_vec_inc {a} (w : mword a) i b : mword a :=
+ opt_def w (update_mword_inc w i b).
 
 (*val update_vec_dec : forall 'a. Size 'a => mword 'a -> integer -> bitU -> mword 'a*)
-Definition update_vec_dec {a} : mword a -> Z -> bitU -> mword a := update_mword_dec.
+Definition update_vec_dec {a} (w : mword a) i b : mword a := opt_def w (update_mword_dec w i b).
 
 (*val subrange_vec_inc : forall 'a 'b. Size 'a, Size 'b => mword 'a -> integer -> integer -> mword 'b*)
-Definition subrange_vec_inc {a b} `{ArithFact (b >= 0)} (w: mword a) : Z -> Z -> mword b := subrange_bv_inc w.
+(* TODO: get rid of bogus default *)
+Parameter dummy_vector : forall {n} `{ArithFact (n >= 0)}, mword n.
+Definition subrange_vec_inc {a b} `{ArithFact (b >= 0)} (w: mword a) i j : mword b :=
+  opt_def dummy_vector (of_bits (subrange_bv_inc w i j)).
 
 (*val subrange_vec_dec : forall 'a 'b. Size 'a, Size 'b => mword 'a -> integer -> integer -> mword 'b*)
-Definition subrange_vec_dec {n m} `{ArithFact (m >= 0)} (w : mword n) : Z -> Z -> mword m := subrange_bv_dec w.
+(* TODO: get rid of bogus default *)
+Definition subrange_vec_dec {n m} `{ArithFact (m >= 0)} (w : mword n) i j :mword m :=
+  opt_def dummy_vector (of_bits (subrange_bv_dec w i j)).
 
 (*val update_subrange_vec_inc : forall 'a 'b. Size 'a, Size 'b => mword 'a -> integer -> integer -> mword 'b -> mword 'a*)
-Definition update_subrange_vec_inc {a b} (v : mword a) i j (w : mword b) : mword a := update_subrange_bv_inc v i j w.
+Definition update_subrange_vec_inc {a b} (v : mword a) i j (w : mword b) : mword a :=
+  opt_def dummy_vector (of_bits (update_subrange_bv_inc v i j w)).
 
 (*val update_subrange_vec_dec : forall 'a 'b. Size 'a, Size 'b => mword 'a -> integer -> integer -> mword 'b -> mword 'a*)
-Definition update_subrange_vec_dec {a b} (v : mword a) i j (w : mword b) : mword a := update_subrange_bv_dec v i j w.
+Definition update_subrange_vec_dec {a b} (v : mword a) i j (w : mword b) : mword a :=
+  opt_def dummy_vector (of_bits (update_subrange_bv_dec v i j w)).
 
 Lemma mword_nonneg {a} : mword a -> a >= 0.
 destruct a;
@@ -61,7 +73,7 @@ destruct 1.
 Qed.
 
 (*val extz_vec : forall 'a 'b. Size 'a, Size 'b => integer -> mword 'a -> mword 'b*)
-Definition extz_vec {a b} `{ArithFact (b >= 0)} `{ArithFact (b >= a)} (n : Z) (v : mword a) : mword b.
+Definition extz_vec {a b} `{ArithFact (b >= a)} (n : Z) (v : mword a) : mword b.
 refine (cast_to_mword (Word.zext (get_word v) (Z.to_nat (b - a))) _).
 unwrap_ArithFacts.
 assert (a >= 0). { apply mword_nonneg. assumption. }
@@ -72,7 +84,15 @@ auto with zarith.
 Defined.
 
 (*val exts_vec : forall 'a 'b. Size 'a, Size 'b => integer -> mword 'a -> mword 'b*)
-Definition exts_vec {a b} `{ArithFact (b >= 0)} (n : Z) (v : mword a) : mword b := exts_bv n v.
+Definition exts_vec {a b} `{ArithFact (b >= a)} (n : Z) (v : mword a) : mword b.
+refine (cast_to_mword (Word.sext (get_word v) (Z.to_nat (b - a))) _).
+unwrap_ArithFacts.
+assert (a >= 0). { apply mword_nonneg. assumption. }
+rewrite <- Z2Nat.inj_add; try omega.
+rewrite Zplus_minus.
+apply Z2Nat.id.
+auto with zarith.
+Defined.
 
 Definition zero_extend {a} (v : mword a) (n : Z) `{ArithFact (n >= a)} : mword n := extz_vec n v.
 
@@ -112,7 +132,13 @@ Definition cast_unit_vec := cast_unit_bv
 val vec_of_bit : forall 'a. Size 'a => integer -> bitU -> mword 'a
 Definition vec_of_bit := bv_of_bit*)
 
-Definition vec_of_bits {a} `{ArithFact (a >= 0)} (l:list bitU) : mword a := of_bits l.
+Lemma length_list_pos : forall {A} {l:list A}, length_list l >= 0.
+unfold length_list.
+auto with zarith.
+Qed.
+Hint Resolve length_list_pos : sail.
+
+Definition vec_of_bits (l:list bitU) : mword (length_list l) := opt_def dummy_vector (of_bits l).
 (*
 
 val msb : forall 'a. Size 'a => mword 'a -> bitU
@@ -122,36 +148,41 @@ val int_of_vec : forall 'a. Size 'a => bool -> mword 'a -> integer
 Definition int_of_vec := int_of_bv
 
 val string_of_vec : forall 'a. Size 'a => mword 'a -> string
-Definition string_of_vec := string_of_bv
+Definition string_of_vec := string_of_bv*)
+Definition with_word' {n} (P : Type -> Type) : (forall n, Word.word n -> P (Word.word n)) -> mword n -> P (mword n) := fun f w => @with_word n _ (f (Z.to_nat n)) w.
+Definition word_binop {n} (f : forall n, Word.word n -> Word.word n -> Word.word n) : mword n -> mword n -> mword n := with_word' (fun x => x -> x) f.
+Definition word_unop {n} (f : forall n, Word.word n -> Word.word n) : mword n -> mword n := with_word' (fun x => x) f.
 
+
+(*
 val and_vec : forall 'a. Size 'a => mword 'a -> mword 'a -> mword 'a
 val or_vec  : forall 'a. Size 'a => mword 'a -> mword 'a -> mword 'a
 val xor_vec : forall 'a. Size 'a => mword 'a -> mword 'a -> mword 'a
 val not_vec : forall 'a. Size 'a => mword 'a -> mword 'a*)
-Definition and_vec {n} (w : mword n) : mword n -> mword n := and_bv w.
-Definition or_vec  {n} (w : mword n) : mword n -> mword n := or_bv w.
-Definition xor_vec {n} (w : mword n) : mword n -> mword n := xor_bv w.
-Definition not_vec {n} (w : mword n) : mword n := not_bv w.
+Definition and_vec {n} : mword n -> mword n -> mword n := word_binop Word.wand.
+Definition or_vec  {n} : mword n -> mword n -> mword n := word_binop Word.wor.
+Definition xor_vec {n} : mword n -> mword n -> mword n := word_binop Word.wxor.
+Definition not_vec {n} : mword n -> mword n := word_unop Word.wnot.
 
 (*val add_vec   : forall 'a. Size 'a => mword 'a -> mword 'a -> mword 'a
 val sadd_vec  : forall 'a. Size 'a => mword 'a -> mword 'a -> mword 'a
 val sub_vec   : forall 'a. Size 'a => mword 'a -> mword 'a -> mword 'a
 val mult_vec  : forall 'a 'b. Size 'a, Size 'b => mword 'a -> mword 'a -> mword 'b
 val smult_vec : forall 'a 'b. Size 'a, Size 'b => mword 'a -> mword 'a -> mword 'b*)
-Definition add_vec {n} (w : mword n) : mword n -> mword n := add_bv w.
-Definition sadd_vec {n} (w : mword n) : mword n -> mword n := sadd_bv w.
-Definition sub_vec  {n} (w : mword n) : mword n -> mword n := sub_bv w.
-Definition mult_vec {n} (w : mword n) : mword n -> mword n := mult_bv w.
-Definition smult_vec {n} (w : mword n) : mword n -> mword n := smult_bv w.
+Definition add_vec   {n} : mword n -> mword n -> mword n := word_binop Word.wplus.
+(*Definition sadd_vec  {n} : mword n -> mword n -> mword n := sadd_bv w.*)
+Definition sub_vec   {n} : mword n -> mword n -> mword n := word_binop Word.wminus.
+Definition mult_vec  {n} : mword n -> mword n -> mword n := word_binop Word.wmult.
+(*Definition smult_vec {n} : mword n -> mword n -> mword n := smult_bv w.*)
 
 (*val add_vec_int   : forall 'a. Size 'a => mword 'a -> integer -> mword 'a
 val sadd_vec_int  : forall 'a. Size 'a => mword 'a -> integer -> mword 'a
 val sub_vec_int   : forall 'a. Size 'a => mword 'a -> integer -> mword 'a
 val mult_vec_int  : forall 'a 'b. Size 'a, Size 'b => mword 'a -> integer -> mword 'b
 val smult_vec_int : forall 'a 'b. Size 'a, Size 'b => mword 'a -> integer -> mword 'b*)
-Definition add_vec_int   {a} (w : mword a) : Z -> mword a := add_bv_int w.
+(*Definition add_vec_int   {a} (w : mword a) : Z -> mword a := add_bv_int w.
 Definition sadd_vec_int  {a} (w : mword a) : Z -> mword a := sadd_bv_int w.
-Definition sub_vec_int   {a} (w : mword a) : Z -> mword a := sub_bv_int w.
+Definition sub_vec_int   {a} (w : mword a) : Z -> mword a := sub_bv_int w.*)
 (*Definition mult_vec_int  {a b} : mword a -> Z -> mword b := mult_bv_int.
 Definition smult_vec_int {a b} : mword a -> Z -> mword b := smult_bv_int.*)
 
@@ -221,7 +252,19 @@ Definition mod_vec_int  := mod_bv_int
 Definition quot_vec_int := quot_bv_int
 
 val replicate_bits : forall 'a 'b. Size 'a, Size 'b => mword 'a -> integer -> mword 'b*)
-Definition replicate_bits {a b} `{ArithFact (b >= 0)} (w : mword a) : Z -> mword b := replicate_bits_bv w.
+Fixpoint replicate_bits_aux {a} (w : Word.word a) (n : nat) : Word.word (n * a) :=
+match n with
+| O => Word.WO
+| S m => Word.combine w (replicate_bits_aux w m)
+end.
+Lemma replicate_ok {n a} `{ArithFact (n >= 0)} `{ArithFact (a >= 0)} :
+   Z.of_nat (Z.to_nat n * Z.to_nat a) = n * a.
+destruct H. destruct H0.
+rewrite <- Z2Nat.id; auto with zarith.
+rewrite Z2Nat.inj_mul; auto with zarith.
+Qed.
+Definition replicate_bits {a} (w : mword a) (n : Z) `{ArithFact (n >= 0)} : mword (n * a) :=
+ cast_to_mword (replicate_bits_aux (get_word w) (Z.to_nat n)) replicate_ok.
 
 (*val duplicate : forall 'a. Size 'a => bitU -> integer -> mword 'a
 Definition duplicate := duplicate_bit_bv
@@ -236,8 +279,8 @@ val ulteq_vec : forall 'a. Size 'a => mword 'a -> mword 'a -> bool
 val slteq_vec : forall 'a. Size 'a => mword 'a -> mword 'a -> bool
 val ugteq_vec : forall 'a. Size 'a => mword 'a -> mword 'a -> bool
 val sgteq_vec : forall 'a. Size 'a => mword 'a -> mword 'a -> bool*)
-Definition eq_vec  {n} (w : mword n) : mword n -> bool := eq_bv w.
-Definition neq_vec {n} (w : mword n) : mword n -> bool := neq_bv w.
+Definition eq_vec  {n} (x : mword n) (y : mword n) : bool := Word.weqb (get_word x) (get_word y).
+Definition neq_vec {n} (x : mword n) (y : mword n) : bool := negb (eq_vec x y).
 (*Definition ult_vec   := ult_bv.
 Definition slt_vec   := slt_bv.
 Definition ugt_vec   := ugt_bv.
